per/per_props_top.v
@@ -1,6 +1,8 @@
 (*
 
   Copyright 2014 Cornell University
+  Copyright 2015 Cornell University
+  Copyright 2016 Cornell University
 
   This file is part of VPrl (the Verified Nuprl project).
 
@@ -18,12 +20,15 @@
   along with VPrl.  If not, see <http://www.gnu.org/licenses/>.
 
 
-  Website: http://nuprl.org/html/verification/
+  Websites: http://nuprl.org/html/verification/
+            http://nuprl.org/html/Nuprl2Coq
+            https://github.com/vrahli/NuprlInCoq
+
   Authors: Abhishek Anand & Vincent Rahli
 
 *)
 
-Require Export per_props.
+Require Export per_props_cequiv.
 
 Lemma type_mkc_top {o} : forall lib, @type o lib mkc_top.
 Proof.
@@ -52,8 +57,10 @@ Proof.
 Qed.
 Hint Resolve equality_mkc_top : slow.
 
+
+
 (*
 *** Local Variables:
-*** coq-load-path: ("." "./close/")
+*** coq-load-path: ("." "../util/" "../terms/" "../computation/" "../cequiv/" "../close/")
 *** End:
 *)
